RelationalCalculus/Union.lean
@@ -1,6 +1,9 @@
+
 import RelationalCalculus.Basic
 import RelationalCalculus.Order
 import RelationalCalculus.Eq
+import Mathlib.Tactic
+-- import Lean.Init.SimpLemmas
 open Relation
 
 
@@ -10,93 +13,58 @@ open Relation
 def Relation.union (R : Relation α β) (S : Relation α β) := comp (comp (Relation.split α) (coproduct R S)) (collapse β)
 
 namespace Relation
-infix:50 "∪" => Relation.union
+infixl:50 "∪" => Relation.union
 end Relation
 
 -- We give the direct set-theoretic definition of a union of two relations.
-def Relation.union.pairs_def (R : Relation α β) (S : Relation α β) : Pairs α β  := fun a b => (eval R) a b ∨ (eval S) a b
+def Relation.union_pairs_def (R : Relation α β) (S : Relation α β) : Pairs α β  := fun a b => (eval R) a b ∨ (eval S) a b
 
 -- Proof that the compositional definition of union is equal to the set theoretic definiton.
-theorem Relation.union.eval_eq_pairs (R : Relation α β) (S : Relation α β) : eval (Relation.union R S) = union.pairs_def R S := by
+theorem Relation.union_eval_eq_pairs (R : Relation α β) (S : Relation α β) : eval (Relation.union R S) = union_pairs_def R S := by
 apply funext
 intro a
 apply funext
 intro b
-simp [Relation.eval, union.pairs_def, Relation.union]
-constructor
-intro ⟨c, ⟨c₁, h₁, h₂⟩, h₃⟩
-cases c₁ <;> cases c <;> simp at h₁ h₂ h₃ <;> subst h₁<;> subst h₃
-· exact Or.inl h₂
-· exact Or.inr h₂
-· intro h4
-  cases h4 with
-  | inl h4R =>
-    use Sum.inl b
-    constructor
-    use Sum.inl a
-    constructor
-  | inr hS =>
-    use Sum.inr b
-    constructor
-    use Sum.inr a
-    constructor
+simp [Relation.eval, union_pairs_def, Relation.union]
 
+theorem Relation.union_assoc {R S T : Relation α β} :
+     ((R ∪ S) ∪ T) ≃ (R ∪ (S ∪ T)) := by
+rw [eq_iff_eval_eq]
+simp [union, eq, eval]
+intro a b
+have assoc :=  @or_assoc (R.eval a b) (S.eval a b) (T.eval a b)
+constructor <;> intro h1
+· exact assoc.mp  h1
+· exact assoc.mpr h1
 
-
-
-
-theorem Relation.union.le_left (R S : Relation α β) : R ≤ Relation.union R S := by
+-- A left side of a union is less then or equal to the union it is a part of
+theorem Relation.union_left_le  (R S : Relation α β) : R ≤ Relation.union R S := by
   intros a b h
-  simp [Relation.eval, Relation.union]
-  use Sum.inl b
-  constructor
-  · use Sum.inl a
-  · simp
+  simp [union, eval]
+  use Or.inl h
 
-theorem Relation.union.le_right (R S : Relation α β) : S ≤ Relation.union R S := by
+-- -- A right side of a union is less then or equal to the union it is a part of
+theorem Relation.union_right_le   (R S : Relation α β) : R ≤ Relation.union S R := by
   intros a b h
-  simp [Relation.eval, Relation.union]
-  use Sum.inr b
-  constructor
-  · use Sum.inr a
-  · simp
+  simp [union, eval]
+  use Or.inr h
 
-theorem Relation.union.le_trans {R S T : Relation α β} (hR : R ≤ T) (hS : S ≤ T) : Relation.union R S ≤ T := by
+-- Union of two lesser relations is lesser, i.e., union preserves ordering
+theorem Relation.union_le {R S T : Relation α β} (hR : R ≤ T) (hS : S ≤ T) : Relation.union R S ≤ T := by
   intros a b h
   simp [Relation.eval, Relation.union] at h
-  rcases h with ⟨c, ⟨d, hd, hc⟩, hb⟩
-  cases d
-  case inl d' =>
-    cases c
-    case inl c' =>
-      simp at hc hb
-      subst hb
-      subst hd
-      exact hR _ _ hc
-    case inr _ => contradiction
-  case inr d' =>
-    cases c
-    case inl _ => contradiction
-    case inr c' =>
-      simp at hc hb
-      subst hb
-      subst hd
-      exact hS _ _ hc
+  rcases h with aRb | aSb
+  · exact hR a b aRb
+  · exact hS a b aSb
 
 
--- -- TODO
--- theorem Relation.union.comm  {α β : Type u } {R S : Relation α β } : (union S R) ≃ (union R S)   := by
---   apply eq_iff_eval_eq.2
---   intro a b
---   simp [union, eval]
---   constructor
---   intro h
---   rcases h with ⟨c, ⟨c₁, h₁, h₂⟩, h₃⟩
---   cases c₁ <;> cases c <;> simp at h₁ h₂ h₃ <;> subst h₁<;> subst h₃
-
-
-
--- -- TODO
--- theorem Relation.union.assoc {R S T : Relation α β} :
---     union (union R S) T ≃ union R (union S T) := by
---     := sorry
+-- Proof that union is commutative.
+theorem Relation_union_comm  {α β : Type u } {R S : Relation α β } : (S ∪ R) ≃ (R ∪ S) := by
+simp [eq]
+have RLeft :  R ≤ (R ∪ S) := union_left_le R S
+have RRight :  R ≤ (S ∪ R) := union_right_le R S
+have SLeft :  S ≤ (S ∪ R) := union_left_le S R
+have SRight :  S ≤ (R ∪ S) := union_right_le S R
+have SR_le_RS := union_le  SRight RLeft
+have RS_le_SE := union_le RRight SLeft
+exact ⟨SR_le_RS, RS_le_SE⟩
