RelationalCalculus/Utility.lean
@@ -1,0 +1,35 @@
+import Mathlib.Tactic
+universe u v
+
+namespace Utility
+
+@[reducible]
+def typeof {α : Sort u} (_:α) := α
+
+
+--- VECT ---
+inductive Vect :  Type u -> Nat -> Type (u+1) :=
+ | emptyV (α:Type u) : Vect α 0
+ | consV {n : Nat } (a: α) (v: Vect α n): Vect α (n + 1)
+
+
+def Vect.toList :  Vect α n → List α
+  | emptyV α  => ([] : List α)
+  | consV a v2 => a :: toList v2
+
+
+instance [Repr α] : Repr (Vect α n) where
+  reprPrec v _ :=
+    let list := v.toList
+    let listRepr := repr list
+    let len := repr n
+    s!"{listRepr} : Vect " ++ len
+
+end Utility
+
+namespace List
+open Utility
+def List.toVect : (l : List α) → Vect α l.length
+  | [] => Vect.emptyV α
+  | (h :: t) => Vect.consV h (toVect t)
+end List
